proof/xarrays/XArray40.ec
@@ -1,5 +1,5 @@
 (* -------------------------------------------------------------------- *)
-require import AllCore List IntDiv JWordExtra CircuitBindings.
+require import AllCore List IntDiv JWordExtra CircuitBindings CircuitBindingsExtra.
 from JazzEC require import Array40.
 
 from Jasmin require import JWord.
@@ -28,3 +28,26 @@ clone BSWA as BSWA_40u16 with
   theory WE    <- WE16,
   theory BSW   <- BSW16
   proof *.
+
+(* -------------------------------------------------------------------- *)
+clone BSWAS as BSWAS_40u16_128 with
+      op asize   <- 40,
+      op bsize   <- 16,
+      op ssize   <- 128,
+  theory A       <- Array40,
+  theory BSA     <- BSA40,
+  theory WB      <- W16  { rename "_XX" as "_16" },
+  theory WEB     <- WE16,
+  theory BSWB    <- BSW16,
+  theory WS      <- W128  { rename "_XX" as "_128" },
+  theory WES     <- WE128,
+  theory BSWS    <- BSW128,
+  theory BSWA    <- BSWA_40u16
+
+  proof le_size by done.
+
+clone export SliceSet as SliceSet_16_128_40
+  with op isize <- 16, op osize <- 128, op asize <- 40,
+  theory IW <- W16, theory OW <- W128, theory A <- Array40
+  rename "XX" as "16_128_40"
+  proof gt0_isize by done, gt0_osize by done, ge0_asize by done.
