proof/xarrays/XArray48.ec
@@ -29,3 +29,36 @@ clone BSWA as BSWA_48u8 with
   theory WE    <- WE8,
   theory BSW   <- BSW8
   proof *.
+
+(* -------------------------------------------------------------------- *)
+clone BSWAS as BSWAS_48u8_12 with
+      op asize   <- 48,
+      op bsize   <- 8,
+      op ssize   <- 12,
+  theory A       <- Array48,
+  theory BSA     <- BSA48,
+  theory WB      <- W8  { rename "_XX" as "_8" },
+  theory WEB     <- WE8,
+  theory BSWB    <- BSW8,
+  theory WS      <- W12  { rename "_XX" as "_12" },
+  theory WES     <- WE12,
+  theory BSWS    <- BSW12,
+  theory BSWA    <- BSWA_48u8
+
+  proof le_size by done.
+
+require import BitEncoding.
+import Array48 BitChunking.
+
+lemma BSWAS_48u8_12_initE (a : W8.t Array48.t) o :
+    0 <= o <= 48*8 - 12 =>
+    BSWAS_48u8_12.sliceget a o = W12.init (fun j => a.[(o + j) %/ 8].[(o + j) %% 8]).
+  proof.
+  move => Ho; apply W12.wordP => k kb; rewrite initiE 1:/# /=.
+  have //= := BSWAS_48u8_12.BVA_asliceget_Top_CircuitBindings_BSWAS_WB_t_Top_CircuitBindings_BSWAS_WS_t_Top_CircuitBindings_BSWAS_A_t.bvaslicegetP a o _ k _; 1,2: by smt().
+  move => ->.
+  rewrite nth_take 1,2:/# nth_drop 1,2:/# (nth_flatten false 8).
+  + rewrite allP /= => x; rewrite mapP => He; elim He; smt(W8.size_w2bits).
+  rewrite (nth_map witness); 1: by rewrite size_to_list; smt().
+  by rewrite get_to_list get_w2bits /#.
+ qed.
