proof/xarrays/XArray56.ec
@@ -28,3 +28,36 @@ clone BSWA as BSWA_56u8 with
   theory WE    <- WE8,
   theory BSW   <- BSW8
   proof *.
+
+(* -------------------------------------------------------------------- *)
+clone BSWAS as BSWAS_56u8_256 with
+      op asize   <- 56,
+      op bsize   <- 8,
+      op ssize   <- 256,
+  theory A       <- Array56,
+  theory BSA     <- BSA56,
+  theory WB      <- W8  { rename "_XX" as "_8" },
+  theory WEB     <- WE8,
+  theory BSWB    <- BSW8,
+  theory WS      <- W256  { rename "_XX" as "_256" },
+  theory WES     <- WE256,
+  theory BSWS    <- BSW256,
+  theory BSWA    <- BSWA_56u8
+
+  proof le_size by done.
+
+require import BitEncoding.
+import Array56 BitChunking.
+
+lemma BSWAS_56u8_256_initE (a : W8.t Array56.t) o :
+    0 <= o <= 56*8 - 256 =>
+    BSWAS_56u8_256.sliceget a o = W256.init (fun j => a.[(o + j) %/ 8].[(o + j) %% 8]).
+  proof.
+  move => Ho; apply W256.wordP => k kb; rewrite initiE 1:/# /=.
+  have //= := BSWAS_56u8_256.BVA_asliceget_Top_CircuitBindings_BSWAS_WB_t_Top_CircuitBindings_BSWAS_WS_t_Top_CircuitBindings_BSWAS_A_t.bvaslicegetP a o _ k _; 1,2: by smt().
+  move => ->.
+  rewrite nth_take 1,2:/# nth_drop 1,2:/# (nth_flatten false 8).
+  + rewrite allP /= => x; rewrite mapP => He; elim He; smt(W8.size_w2bits).
+  rewrite (nth_map witness); 1: by rewrite size_to_list; smt().
+  by rewrite get_to_list get_w2bits /#.
+ qed.
