proof/xarrays/XArray32.ec
@@ -122,3 +122,16 @@ clone export A2B as A2B_8_256_32
 bind op [W256.t & W8.t & Array32.t] u8_256_32 "a2b".
 realize a2bP by apply/u8_256_32P.
 realize size_ok by auto.
+
+lemma BSWAS_32u8_256_initE (a : W8.t Array32.t) o :
+    0 <= o <= 32*8 - 256 =>
+    BSWAS_32u8_256.sliceget a o = W256.init (fun j => a.[(o + j) %/ 8].[(o + j) %% 8]).
+  proof.
+  move => Ho; apply W256.wordP => k kb; rewrite initiE 1:/# /=.
+  have //= := BSWAS_32u8_256.BVA_asliceget_Top_CircuitBindings_BSWAS_WB_t_Top_CircuitBindings_BSWAS_WS_t_Top_CircuitBindings_BSWAS_A_t.bvaslicegetP a o _ k _; 1,2: by smt().
+  move => ->.
+  rewrite nth_take 1,2:/# nth_drop 1,2:/# (nth_flatten false 8).
+  + rewrite allP /= => x; rewrite mapP => He; elim He; smt(W8.size_w2bits).
+  rewrite (nth_map witness); 1: by rewrite size_to_list; smt().
+  by rewrite get_to_list get_w2bits /#.
+ qed.
